# Forward Elimination


    x  + 2y + z =   2
    3x + 8y + z =  12 
         4y + z =   2 


    [1] 2  1
     3  8  1   
     0  4  1

3 is the first pivot, so multiple coeffs in first row by 3 and subtract from 2nd row to eliminate the 3 coeff in 2nd row

    
    x             y            z
    3 - (1 * 3 ), 8 - (2 * 3), 1 - (1 * 3)

     1  2  1  
     0  2 -2
     0  4  1


Now, there's already a 0 in the 3rd equation's x, so no forward elimination step needed there.

Next, to eliminate the 4, 2 is our next pivot

    y            z
    4 - (2 * 2), 1 - (2 * -2)
    
    1  2  1
    0  2 -2
    0  0  5

Our pivots are [3, 2]

    U is [1,2,5]
    c is [2,6,-10]  which was generated by taking the pivots against [ 2 12 2 ], the rhs above
    
    | 2|                   |2|                        |  2|            |  2|
    |12 - (2 * 3)|         |6|  second pivot is 2  =  |  6|         =  |  6|
    | 2 (stays the same|   |2|                        |2 - (6\*2)|     |-10|

## Elimination matrics
  
    E(2,1) 
      | 1 0 0|   |1 2 1|   |1  2  1|
      |-3 1 0| * |3 8 1| = |0  2 -2|
      | 0 0 1|   |0 4 1|   |0  4  1|


    E(3,2) 
      | 1  0 0|   |1 2  1|   |1  2  1|
      | 0  1 0| * |0 2 -2| = |0  2 -2|
      | 0 -2 1|   |0 4  1|   |0  0  5|

So,

      E(3,2)  ( E(2,1) * A ) = U
     
        == 

      (E(3,2) * E(2,1) )  * A = U


# Back Substitution

Rewrite equations with forward-eliminated matrix and c,

    x + 2y +  z =   2
        2y - 2z =   6
             5z = -10
    
Now just solve the equations manually, starting from bottom:

    5z = -10, so, z = -2

Substitute z = -2 into next equation upwards,

    2y - (2 * -2) = 6
    2y = 2
     y = 1

And finally with first equation and y = 1, and z = -2

    x + (2*1) - 2 = 2
    x = 2

